theories/leb128.v
@@ -8,11 +8,11 @@ From parseque Require Import Parseque.
 
 (** expects 7 bits, with MSB at head *)
 Definition byte_of_7_bits (bs : list bool) : byte :=
-  (* TODO: using lists is very inefficient *)
+  (* using lists is very inefficient *)
   match bs with
   | cons b1 (cons b2 (cons b3 (cons b4 (cons b5 (cons b6 (cons b7 nil)))))) =>
     Byte.of_bits (b7, (b6, (b5, (b4, (b3, (b2, (b1, false)))))))
-  | _ => (* TODO: should never happen *) x00
+  | _ => (* should never happen *) x00
   end.
 
 Definition rebalance (bytes_produced : list byte) (bits_produced : list bool) (the_bit : bool) :
@@ -20,19 +20,52 @@ Definition rebalance (bytes_produced : list byte) (bits_produced : list bool) (t
   if Nat.eqb (List.length bits_produced) 6 then (cons (byte_of_7_bits (cons the_bit bits_produced)) bytes_produced, nil)
   else (bytes_produced, cons the_bit bits_produced).
 
-Fixpoint binary_of_aux2 (is_neg : bool) (acc1 : list byte) (acc2 : list bool (* MSB at head *)) (n : positive) : list byte :=
-  (* TODO: using lists is very inefficient *)
+Fixpoint binary_of_aux2 (acc1 : list byte) (acc2 : list bool (* MSB at head *)) (n : positive) : list byte :=
+  (* using lists is very inefficient *)
   match n with
   | xH =>
     let (acc1', acc2') := rebalance acc1 acc2 true in
-    let acc2'' := List.app (List.repeat is_neg (7 - List.length acc2')) acc2' in
+    let acc2'' := List.app (List.repeat false (6 - List.length acc2)) acc2' in
     cons (byte_of_7_bits acc2'') acc1'
   | xI n' =>
     let (acc1', acc2') := rebalance acc1 acc2 true in
-    binary_of_aux2 is_neg acc1' acc2' n'
+    binary_of_aux2 acc1' acc2' n'
   | xO n' =>
     let (acc1', acc2') := rebalance acc1 acc2 false in
-    binary_of_aux2 is_neg acc1' acc2' n'
+    binary_of_aux2 acc1' acc2' n'
+  end.
+
+Definition incr_mod (len: nat) (pad: nat) : nat :=
+  if Nat.eqb (S len) pad then 0 else (S len).
+
+(* Convert pos to bits, MSB at head *)
+Fixpoint bits_of_pos_pad (acc: list bool) (len: nat) (pad: nat) (n: positive) : list bool :=
+  match n with
+  | xH =>
+    List.app (List.repeat false (pad - 1 - len)) (cons true acc)
+  | xI n' =>
+    bits_of_pos_pad (cons true acc) (incr_mod len pad) pad n'
+  | xO n' =>
+    bits_of_pos_pad (cons false acc) (incr_mod len pad) pad n'
+  end.
+
+(* Evaluate two's complement LEB128 encoding. Need LSB at head *)
+Fixpoint complement_of_one_two_aux (zeros: nat) (bs: list bool) : list bool :=
+  match bs with
+  | nil => List.repeat false zeros
+  | cons true bs' => List.app (List.repeat false zeros) (cons true (List.map negb bs'))
+  | cons false bs' => complement_of_one_two_aux (S zeros) bs'
+  end.
+
+(* MSB at head *)
+Definition complement_of_one_two (bs: list bool) : list bool :=
+  List.rev (complement_of_one_two_aux 0 (List.rev bs)).
+
+Fixpoint bytes_of_bits (bs: list bool): list byte :=
+  match bs with
+  | cons b1 (cons b2 (cons b3 (cons b4 (cons b5 (cons b6 (cons b7 bs')))))) =>
+    cons (Byte.of_bits (b7, (b6, (b5, (b4, (b3, (b2, (b1, false)))))))) (bytes_of_bits bs')
+  | _ => (* should never happen *) nil
   end.
 
 Definition make_msb_one (b : byte) : byte :=
@@ -53,7 +86,7 @@ Definition make_msb_of_non_first_byte_one (bs : list byte) : list byte :=
 Definition encode_unsigned_aux (n : N) : list byte :=
   match n with
   | N0 => cons x00 nil
-  | Npos n' => make_msb_of_non_first_byte_one (binary_of_aux2 false nil nil n')
+  | Npos n' => make_msb_of_non_first_byte_one (binary_of_aux2 nil nil n')
   end.
 
 Definition encode_unsigned (n : N) : list byte :=
@@ -62,8 +95,11 @@ Definition encode_unsigned (n : N) : list byte :=
 Definition encode_signed_aux (z : Z) : list byte :=
   match z with
   | Z0 => cons x00 nil
-  | Zpos n' => make_msb_of_non_first_byte_one (binary_of_aux2 false nil nil n')
-  | Zneg n' => make_msb_of_non_first_byte_one (binary_of_aux2 true nil nil n')
+  | Zpos n' => make_msb_of_non_first_byte_one (binary_of_aux2 nil nil n')
+  | Zneg n' => make_msb_of_non_first_byte_one
+                (bytes_of_bits
+                   (complement_of_one_two
+                      (bits_of_pos_pad nil 0 7 n')))
   end.
 
 Definition encode_signed (z : Z) : list byte :=
